\documentclass{ximera}

\input{../preamble.tex}

\title{Nakayama's lemma}

\begin{document}
\begin{abstract}
  We introduce and prove Nakayama's lemma. Sources and references:
  \cite{AM1969,jpS2000}.
\end{abstract}
\maketitle

We start by introducing the \textit{Jacobson radical}, an ideal related to the nilradical.

\begin{definition}\index{JA@$\i J(A)$}
  If $R$ is a ring we define the \dfn{Jacobson radical} to be
  \[
  \i J(R) := \bigcap_{\m \text{ maximal}}\m.
  \]
\end{definition}

\begin{exercise}
  Prove that the Jacobson radical is an ideal.
\end{exercise}

\begin{proposition}\label{P:CharJR}
  Let $R$ be a ring, $j\in\i J(R)$ if and only if $1-jr$ is a unit in
  $R$ for all $r\in R$.
  \begin{proof}
    $(\Rightarrow)$ Seeking a contradiction, suppose that $j\in \i
    J(R)$ but $1-jr$ is not a unit in $R$. There is a maximal ideal
    $\m$ such that $1-jr\in\m$. However, $j\in\m$, implying that
    $jr\in\m$, and hence $1\in\m$. This would mean that $\m = R$, a
    contradiction.

    $(\Leftarrow)$ Suppose that $j\notin\i J(R)$, hence there is some
    maximal ideal $\m$ such that $j\notin\m$. Now, $(j)+\m = R$, so
    there is $r\in\R$ and $m\in\m$ such that $jr+m = 1$. This means
    $1-jr\in\m$ and cannot be a unit.
  \end{proof}
\end{proposition}

\begin{exercise}
  Let $R$ be a ring. Show that $\rad{0}\subset \i J(R)$.
\end{exercise}

\begin{exercise}
  Let $R$ be a ring and consider $R[X]$. Show that $\rad{0_{R[X]}} =
  \i J(R)$.
\end{exercise}





We now introduce the ``determinant trick.''

\begin{proposition}[Determinant trick]\label{P:determinanttrick}
  Let $M$ be a finitely generated $R$-module and $I\subset R$ an ideal
  of $R$. If $\phi:M\to M$ is an $R$-module homomorphism such that
  $\phi(M)\subset I M$, then $\phi$ satisfies and equation of the form
  \[
  \phi^n(x) + a_{n-1}\phi^{n-1}(x) + \dots + a_1 \phi(x)  + a_0 = 0.
  \]
  for all $x\in M$ and $a_i\in I$.
  \begin{proof}
    Let $\{m_1,\dots, m_n\}$ be a set of generators for $M$. Hence $\phi(m_i) \in I M$. Letting $a_{i,j}\in I$, we may write this:
    \begin{align*}
      \phi(m_1) &= a_{1,1}m_1 + a_{1,2}m_2 + \dots + a_{1,n}m_n\\
      \phi(m_2) &= a_{2,1}m_1 + a_{2,2}m_2 + \dots + a_{2,n}m_n\\
      &\hspace{.5em}  \vdots \\
      \phi(m_n) &= a_{n,1}m_1 + a_{n,2}m_2 + \dots + a_{n,n}m_n. 
    \end{align*}
    We can express this relationship as the following matrix equation:
    \[
    \begin{bmatrix}
      \phi - a_{1,1} & - a_{1,2} & \cdots & - a_{1,n}\\
      - a_{2,1} & \phi - a_{2,2} & \cdots & - a_{2,n}\\
      \vdots & \vdots & & \vdots \\
      -a_{n,1} & -a_{n,2} & \cdots & \phi - a_{n,n}
    \end{bmatrix}
    \begin{bmatrix}
      m_1\\
      m_2\\
      \vdots \\
      m_n
    \end{bmatrix}
    =
    \begin{bmatrix}
      0\\
      0\\
      \vdots\\
      0
    \end{bmatrix}
    \]
    Let $X$ be the $n \times n$ matrix shown.  Let $Y_i$ be the
    identity $n \times n$ matrix with the $i$th column replaced by the
    column in the above equation with entries $m_1,\dots,m_n$.  Then
    by the above equation, the $i$th column in the product $X\cdot
    Y_i$ will be the $0$ column for all $i$.  Thus $\det(X\cdot Y_i)
    =0$.  Therefore
    \[
    \det(X) m_i = \det(X) \det(Y_i) = \det(X \cdot Y_i) = 0.
    \]
    This means that $\det(X)$ is the zero endomorphism of
    $M$. Computing the determinant gives an equation of the desired
    form.
  \end{proof}
\end{proposition}

\begin{corollary}
  Let $R$ be a ring, $M$ be a finitely generated $R$-module, and
  $I\subset R$ be an ideal of $R$ such that $IM = M$. Then there is
  $x$ comaximal to $I$ such that $xM = 0$.
  \begin{proof}
    In the proposition above, set $\phi$ to be the identity map, and
    so for any $m\in M$,
    \[
    m + m a_{n-1} + \dots + m a_1 + m a_0 = 0.
    \]
    We set $x = 1 + a_{n-1} + \dots + a_1 + a_0$.
  \end{proof}
\end{corollary}

%% \begin{corollary}[Nakayama's lemma]
%%   Let $R$ be a ring, $M$ be a finitely generated $R$-module, and
%%   $I\subset R$ be an ideal with $I\subset \i J(R)$. In this case
%%   \[
%%   IM = M \quad\Rightarrow\quad M = 0.
%%   \]
%%   \begin{proof}
%%     By the corollary above, there exists $x$ comaximal to $\i J(R)$
%%     such that $xM = 0$. This means
%%     \begin{align*}
%%       xy + j &= 1\\
%%       xy &= 1-j,
%%     \end{align*}
%%     but $1-j$ is a unit by Proposition~\ref{P:CharJR}, hence $x$ is a
%%     unit. Thus $M = x^{-1}x M = 0$.
%%   \end{proof}
%% \end{corollary}

%% \begin{corollary}
%%   Let $R$ be a ring, $I\subset R$ be an ideal of $R$ with $I\subset \i
%%   J(R)$, $M$ be a finitely generated $R$-module, and $N\subset M$ a
%%   submodule of $M$. In this case
%%   \[
%%   M = IM + N \quad \Rightarrow \quad M = N.
%%   \]
%%   \begin{sketch}
%%     Apply Nakayama's lemma to $(M/N)$ and note by an isomorphism
%%     theorem that $I(M/N)\iso (IM + N)/N$.
%%   \end{sketch}
%% \end{corollary}

%% \begin{exercise}
%%   Let $(A,\m)$ be a local ring and $M$ a finitely generated
%%   $A$-module. Show that $M/\m M$ is a finitely generated $A/\m$-vector space.
%% \end{exercise}


%% We now come to an important fact when studying finitely generated
%% modules over local rings.

%% \begin{corollary}
%%   Let $(A,\m)$ be a local ring and $M$ a finitely generated
%%   $A$-module. Consider the canonical surjection
%%   \[
%%   M \to  M/\m M
%%   \]
%%   If $\{\bar{m}_1,\dots, \bar{m}_n\}$ form a basis for the $A/\m$-vector
%%   space $M/\m M$, then $\{m_1,\dots, m_n\}$ generate $M$.
%%   \begin{proof}
%%     The map
%%     \[
%%     \sum_{i=1}^n m_iA \to M \to M/\m M
%%     \]
%%     maps $\{m_1,\dots, m_n\}A$ onto $M/\m M$, so
%%     \[
%%     M = \m M + \sum_{i=1}^n m_iA 
%%     \]
%%     and $M = \sum_{i=1}^n m_iA$ by the corollary above.
%%   \end{proof}
%% \end{corollary}


\begin{theorem}[Nakayama's lemma]
  Let $R$ be a ring $M$ be a finitely generated $R$-module. The
  following are equivalent:
  \begin{enumerate}
    \item Let $I\subset R$ be an ideal of $R$ such that $IM = M$. Then
      there is $x$ comaximal to $I$ such that $xM = 0$.
    \item Let $I\subset \i J(R)$ be an ideal of $R$. In this case
      \[
      IM = M \quad\Rightarrow\quad M = 0.
      \]
    \item $I\subset \i J(R)$ be an ideal of $R$ and $N\subset M$ a
      submodule of $M$. In this case
      \[
      M = IM + N \quad \Rightarrow \quad M = N.
      \]
    \item Let $(A,\m)$ be a local ring and $M$ a finitely generated
      $A$-module. Consider the canonical surjection
      \[
      M \to  M/\m M.
      \]
      If $\{\bar{m}_1,\dots, \bar{m}_n\}$ form a basis for the $A/\m$-vector
      space $M/\m M$, then $\{m_1,\dots, m_n\}$ generate $M$.
  \end{enumerate}
  \begin{proof} 
    (a)$\Rightarrow$(b) There exists $x$ comaximal to $\i J(R)$ such
    that $xM = 0$. This means
    \begin{align*}
      xy + j &= 1\\
      xy &= 1-j,
    \end{align*}
    but $1-j$ is a unit by Proposition~\ref{P:CharJR}, hence $x$ is a
    unit. Thus $M = x^{-1}x M = 0$.

    
    (b)$\Rightarrow$(c) Apply Nakayama's lemma to $(M/N)$ and note by
    an isomorphism theorem that $I(M/N)\iso (IM + N)/N$.

    
    (c)$\Rightarrow$(d) The map
    \[
    \sum_{i=1}^n m_iA \to M \to M/\m M
    \]
    maps $\{m_1,\dots, m_n\}A$ onto $M/\m M$, so
    \[
    M = \m M + \sum_{i=1}^n m_iA 
    \]
    and $M = \sum_{i=1}^n m_iA$ by the corollary above.

    
    (d)$\Rightarrow$(a) Suppose that $x$ is comaximal to $I$, hence
    \begin{align*}
      x + I &= R
      xM + IM &= M
    \end{align*}
    Localize at $\m$, where $I\subset\m$
    \[
    xM_\m + I_\m M_\m = M_\m
    \]
    and mod out by $\m$,
    \[
    \frac{xM_\m + I_\m M_\m}{\m M_\m} = M_\m/\m M_\m
    \]
    since this is a $R_\m/\m R_\m$-vector space, we may break up the sum to see
    \[
    xM_\m/\m M_\m + I_\m M_\m/\m M_\m = M_\m/\m M_\m
    \]
    however, since $I\subset\m$ and $M = IM$ we have
    \[
    xM_\m/\m M_\m =0.
    \]
    Since $x$ is comaximal with $\m$, this means $xM = 0$.
  \end{proof}
\end{theorem}


\section{Applications}

\begin{corollary}
  Let $(A,\m)$ be a local ring, then
  \[
  \bigcap_{n\ge 1} \m^n  = (0)
  \]
  \begin{proof}
    Set $I = \bigcap_{n\ge 1} \m^n$. We will show that $\m I = I$, and
    hence by Nakayama, $I = (0)$.

    $(\subset)$ It is clear that $\m I \subset I$.

    $(\supset)$ We must show $I\subset \m I$. Consider a primary
    decomposition of $\m I$
    \[
    \m I = \bigcap_{i=1}^n \q_i.
    \]
    Let $\ass(A/\q_i) = \{\p\}$. Now consider
    \begin{align*}
      x &\in I -\p\\
      y &\in \m = \p.
    \end{align*}
    From this we have $ab\in\m I \subset \q_i$. Hence $ab\in\ann(a)$
    for some $a\in A/\q_i$, which means $ab\in \p$, a contradiction.

    Now if $\ass(A/\q_i) = \m$, then $\m^n\in\q_i$, hence $I\in\q_i$,
    and so $I\subset \m I$.
  \end{proof}
\end{corollary}








\end{document}
